backend/Deadcodeproof.v
@@ -16,7 +16,7 @@ Require Import FunInd.
 Require Import Coqlib Maps Errors Integers Floats Lattice Kildall.
 Require Import AST Linking.
 Require Import Values Memory Globalenvs Events Smallstep.
-Require Import LanguageInterface Invariant.
+Require Import LanguageInterface Invariant cklr.Extends.
 Require Import Registers Op RTL.
 Require Import ValueDomain ValueAnalysis NeedDomain NeedOp Deadcode.
 
@@ -1079,10 +1079,10 @@ Ltac UseTransfer :=
 Qed.
 
 Lemma transf_initial_states:
-  forall q1 q2 st1, cc_ext_query q1 q2 -> initial_state ge q1 st1 ->
+  forall w q1 q2 st1, match_query (cc_c ext) w q1 q2 -> initial_state ge q1 st1 ->
   exists st2, initial_state tge q2 st2 /\ match_states st1 st2.
 Proof.
-  intros. destruct H. inv H0.
+  intros. destruct H. inv H0. CKLR.uncklr. destruct H as [vf|]; try congruence.
   exploit functions_translated; eauto. intros (tf & A & B).
   exists (Callstate nil vf vargs2 m2); split.
   setoid_rewrite <- (sig_function_translated _ _ _ B). monadInv B.
@@ -1091,17 +1091,18 @@ Proof.
 Qed.
 
 Lemma transf_final_states:
-  forall st1 st2 r1, match_states st1 st2 -> final_state st1 r1 ->
-  exists r2, final_state st2 r2 /\ cc_ext_reply r1 r2.
+  forall w st1 st2 r1, match_states st1 st2 -> final_state st1 r1 ->
+  exists r2, final_state st2 r2 /\ match_reply (cc_c ext) w r1 r2.
 Proof.
   intros. inv H0. inv H. inv STACKS.
-  eexists. split; constructor; auto.
+  eexists. split. constructor; auto.
+  exists tt; split; constructor; CKLR.uncklr; auto.
 Qed.
 
 Lemma transf_external_states:
   forall st1 st2 q1, match_states st1 st2 -> at_external ge st1 q1 ->
-  exists q2, at_external tge st2 q2 /\ cc_ext_query q1 q2 /\ se = se /\
-  forall r1 r2 st1', cc_ext_reply r1 r2 -> after_external st1 r1 st1' ->
+  exists q2, at_external tge st2 q2 /\ match_query (cc_c ext) tt q1 q2 /\ se = se /\
+  forall r1 r2 st1', match_reply (cc_c ext) tt r1 r2 -> after_external st1 r1 st1' ->
   exists st2', after_external st2 r2 st2' /\ match_states st1' st2'.
 Proof.
   intros st1 st2 q1 Hst Hq1. destruct Hq1. inv Hst.
@@ -1109,9 +1110,9 @@ Proof.
   eexists. intuition idtac.
   - monadInv TFD. econstructor; eauto.
   - destruct VF; try discriminate.
-    constructor; auto.
+    constructor; CKLR.uncklr; auto.
     destruct v; cbn in *; congruence.
-  - inv H1. inv H0.
+  - inv H1. destruct H0 as ([ ] & _ & H0). inv H0. CKLR.uncklr.
     exists (Returnstate ts vres2 m2); split; constructor; eauto.
 Qed.
 
@@ -1121,12 +1122,13 @@ End PRESERVATION.
 
 Theorem transf_program_correct prog tprog:
   match_prog prog tprog ->
-  forward_simulation (vamatch @ cc_ext) (vamatch @ cc_ext) (RTL.semantics prog) (RTL.semantics tprog).
+  forward_simulation (vamatch @ cc_c ext) (vamatch @ cc_c ext) (RTL.semantics prog) (RTL.semantics tprog).
 Proof.
   intros MATCH. eapply source_invariant_fsim; eauto using rtl_vamatch. revert MATCH.
   fsim eapply forward_simulation_step with (match_states := match_states prog se1);
     cbn in *; subst.
-- destruct 1. cbn. eapply (Genv.is_internal_transf_partial_id MATCH).
+- destruct 1. cbn. CKLR.uncklr. destruct H as [vf|]; try congruence.
+  eapply (Genv.is_internal_transf_partial_id MATCH).
   intros [|] [|] TFD; monadInv TFD; auto.
 - intros q1 q2 s1 Hq (Hs1 & _).
   eapply transf_initial_states; eauto.
