backend/Tailcallproof.v
@@ -15,6 +15,7 @@
 Require Import Coqlib Maps Integers AST Linking.
 Require Import Values Memory Events Globalenvs LanguageInterface Smallstep.
 Require Import Op Registers RTL Conventions Tailcall.
+Require Import cklr.Extends.
 
 (** * Syntactic properties of the code transformation *)
 
@@ -549,10 +550,11 @@ Proof.
 Qed.
 
 Lemma transf_initial_states:
-  forall q1 q2 st1, cc_ext_query q1 q2 -> initial_state ge q1 st1 ->
+  forall w q1 q2 st1, match_query (cc_c ext) w q1 q2 -> initial_state ge q1 st1 ->
   exists st2, initial_state tge q2 st2 /\ match_states st1 st2.
 Proof.
-  intros. destruct H. inv H0.
+  intros. destruct H. inv H0. CKLR.uncklr.
+  destruct H as [vf | ]; try discriminate.
   exploit functions_translated; eauto. intro FIND.
   exists (Callstate nil vf vargs2 m2); split.
   setoid_rewrite <- (sig_preserved (Internal f)). econstructor; eauto.
@@ -560,17 +562,19 @@ Proof.
 Qed.
 
 Lemma transf_final_states:
-  forall st1 st2 r1, match_states st1 st2 -> final_state st1 r1 ->
-  exists r2, final_state st2 r2 /\ cc_ext_reply r1 r2.
+  forall w st1 st2 r1, match_states st1 st2 -> final_state st1 r1 ->
+  exists r2, final_state st2 r2 /\ match_reply (cc_c ext) w r1 r2.
 Proof.
   intros. inv H0. inv H. inv H3.
-  eexists; split; constructor; auto.
+  eexists; split.
+  - constructor.
+  - exists tt. split; constructor; CKLR.uncklr; cbn; auto.
 Qed.
 
 Lemma transf_external_states:
   forall st1 st2 q1, match_states st1 st2 -> at_external ge st1 q1 ->
-  exists q2, at_external tge st2 q2 /\ cc_ext_query q1 q2 /\ se = se /\
-  forall r1 r2 st1', cc_ext_reply r1 r2 -> after_external st1 r1 st1' ->
+  exists q2, at_external tge st2 q2 /\ match_query (cc_c ext) tt q1 q2 /\ se = se /\
+  forall r1 r2 st1', match_reply (cc_c ext) tt r1 r2 -> after_external st1 r1 st1' ->
   exists st2', after_external st2 r2 st2' /\ match_states st1' st2'.
 Proof.
   intros st1 st2 q1 Hst Hq1. destruct Hq1. inv Hst.
@@ -578,9 +582,9 @@ Proof.
   eexists. intuition idtac.
   - econstructor; eauto.
   - destruct H6; try discriminate.
-    constructor; auto.
+    constructor; CKLR.uncklr; auto.
     destruct v; cbn in *; congruence.
-  - inv H1. inv H0.
+  - inv H1. destruct H0 as ([ ] & [ ] & H0). inv H0. CKLR.uncklr.
     exists (Returnstate s' vres2 m2); split; constructor; eauto.
 Qed.
 
@@ -591,10 +595,11 @@ End PRESERVATION.
 
 Theorem transf_program_correct prog tprog:
   match_prog prog tprog ->
-  forward_simulation cc_ext cc_ext (RTL.semantics prog) (RTL.semantics tprog).
+  forward_simulation (cc_c ext) (cc_c ext) (RTL.semantics prog) (RTL.semantics tprog).
 Proof.
   fsim eapply forward_simulation_opt with (measure := measure); destruct Hse.
-  - destruct 1. cbn. eapply (Genv.is_internal_transf_id MATCH). intros [|]; auto.
+  - destruct 1. CKLR.uncklr. destruct H; try congruence.
+    eapply (Genv.is_internal_transf_id MATCH). intros [|]; auto.
   - eapply transf_initial_states; eauto.
   - eapply transf_final_states; eauto.
   - exists tt. eapply transf_external_states; eauto.
